add 'add operator' soundness

Soundness/Domain.lean
@@ -17,18 +17,6 @@ def γItv : Itv → Set ℤ
 | Itv.bot        => ∅
 | (Itv.mk lo hi _) => {z | lo ≤ z ∧ z ≤ hi}
 
-def add (S T : Set ℤ) : Set ℤ :=
-  {z | ∃ x ∈ S, ∃ y ∈ T, z = x + y}
-
-def add_abs (I J : Itv) : Itv :=
-  match I, J with
-  | Itv.bot, _ => Itv.bot
-  | _, Itv.bot => Itv.bot
-  | Itv.mk lo₁ hi₁ h₁, Itv.mk lo₂ hi₂ h₂ =>
-      Itv.mk (lo₁ + lo₂) (hi₁ + hi₂) (by linarith)
-
-notation I " ⊕ " J => add_abs I J
-
 /-- Concrete locations -/
 abbrev Base := ℤ
 abbrev Offset := ℤ
@@ -39,15 +27,17 @@ structure Loc where
 deriving Repr, DecidableEq
 
 /-- Abstract locations -/
-abbrev Label := Nat
+abbrev ℙ := Nat
 
-structure AbsLoc where
-  allocSite : Label
-  offset : Itv
+inductive AbsLoc where
+| bot
+| mk (allocSite : ℙ) (offset : Itv)
 deriving Repr
 
-def γLoc (env : Label → Set Base) (absℓ : AbsLoc) : Set Loc :=
-  { ℓ : Loc | ℓ.base ∈ env absℓ.allocSite ∧ ℓ.offset ∈ γItv absℓ.offset }
+def γLoc (env : ℙ → Set Base) (absℓ : AbsLoc) : Set Loc :=
+match absℓ with
+| AbsLoc.bot => ∅
+| AbsLoc.mk allocSite offset => { ℓ : Loc | ℓ.base ∈ env allocSite ∧ ℓ.offset ∈ γItv offset }
 
 /-- Concrete Unit -/
 notation "⋅" => ()
@@ -76,8 +66,51 @@ structure AbsValue where
   absunit : AbsUnit
 deriving Repr
 
-def γValue (env : Label → Set Base) (absv : AbsValue) : Set Value :=
+def γValue (penv : ℙ → Set Base) (absv : AbsValue) : Set Value :=
   let intSet := {Value.int z | z ∈ γItv absv.absint}
-  let locSet := {Value.loc ℓ | ℓ ∈ γLoc env absv.absloc}
+  let locSet := {Value.loc ℓ | ℓ ∈ γLoc penv absv.absloc}
   let unitSet := {Value.unit u | u ∈ γUnit absv.absunit}
   intSet ∪ locSet ∪ unitSet
+
+/-- Semantic operators -/
+
+def add (S T : Set ℤ) : Set ℤ :=
+  {z | ∃ x ∈ S, ∃ y ∈ T, z = x + y}
+
+def addVal (S T : Set Value) : Set Value :=
+  { v | ∃ z1 z2,
+      v = Value.int (z1 + z2)
+      ∧ Value.int z1 ∈ S
+      ∧ Value.int z2 ∈ T }
+
+def addAbs_itv (I J : Itv) : Itv :=
+  match I, J with
+  | Itv.bot, _ => Itv.bot
+  | _, Itv.bot => Itv.bot
+  | Itv.mk lo₁ hi₁ h₁, Itv.mk lo₂ hi₂ h₂ =>
+      Itv.mk (lo₁ + lo₂) (hi₁ + hi₂) (by linarith)
+
+notation I " ⊕ " J => addAbs_itv I J
+
+def addAbs (v1 v2 : AbsValue) : AbsValue :=
+  let absint :=
+    match v1.absint, v2.absint with
+    | I, J => I ⊕ J
+  AbsValue.mk absint AbsLoc.bot AbsUnit.bot
+
+-- def equal : Value → Value → Prop
+-- | Value.int z1, Value.int z2 => z1 = z2
+-- | Value.loc ℓ1, Value.loc ℓ2 => ℓ1 = ℓ2
+-- | Value.unit _, Value.unit _ => True
+-- | _, _ => False
+
+-- def eqAbs (v1 v2: AbsValue) : Prop :=
+--   let int_eq := match v1.absint, v2.absint with
+--                  | Itv.bot, _ => False
+--                  | _, Itv.bot => False
+--                  | Itv.mk lo₁ hi₁ h₁, Itv.mk lo₂ hi₂ h₂ =>
+--                      lo₁ = lo₂ ∧ hi₁ = hi₂
+--   let loc_eq := if v1.absloc = AbsLoc.bot ∨ v2.absloc = AbsLoc.bot then False
+--                  else v1.absloc = v2.absloc
+--   let unit_eq := if v1.absunit = AbsUnit.bot ∨ v2.absunit = AbsUnit.bot then False
+--                  else v1.absunit = v2.absunit
